Nova definição de AFD + model-checking de capacidade máxima

DFA.v
@@ -1,71 +1,28 @@
-Require Import Coq.Lists.List.
-Import ListNotations.
-Set Implicit Arguments.
+Require Import Coq.Init.Nat Coq.Lists.List Omega.
+Require BinIntDef.
+Local Open Scope Z_scope.
 
-Inductive state {Q} :=
-  sink_state | proper_state (q : Q).
+Inductive event := add | rem | oth.
 
-Record DFA {Q E} := {
-  transition: Q -> E -> @state Q;
-  initial_state: Q;
-  is_marked: Q -> bool
-}.
-
-Definition is_proper_transition {Q E} (G:@DFA Q E) q e := exists q',
-  proper_state q' = transition G q e.
-
-(* Extended transition function: *)
-
-Fixpoint extended_transition {Q E} (G:@DFA Q E) q w : state :=
-  match q with
-    sink_state => sink_state |
-    proper_state q' =>  match w with
-                          [] => proper_state q' |
-                          e::w' =>
-                            extended_transition G (transition G q' e) w'
-                        end
+Definition count_event e :=
+  match e with
+    add =>  1 |
+    rem => -1 |
+    oth =>  0
   end.
 
-Lemma extended_transition__transition: forall {Q E} {G:@DFA Q E} q e,
-  extended_transition G (proper_state q) [e] = transition G q e.
-Proof.
-  intros Q E G q e.
-  simpl.
-  destruct (transition G q e); reflexivity.
-Qed.
+Definition states_num := 6%nat.
+(* Axiom states_num : nat. *)
 
-Lemma transition_sink_state: forall {Q E} (G:@DFA Q E) w,
-  extended_transition G sink_state w = sink_state.
-Proof.
-  intros Q E G w.
-  destruct w; reflexivity.
-Qed.
-
-Theorem dist_extended_transition: forall {Q E} (G:@DFA Q E) w w' q,
-    extended_transition G q (w ++ w') =
-    extended_transition G (extended_transition G q w) w'.
-Proof.
-  intros Q E G w.
-  induction w as [|e w IHw].
-  - intros w' q. simpl. destruct q; reflexivity.
-  - intros w' q. simpl. destruct q.
-    + symmetry. apply transition_sink_state.
-    + rewrite IHw. reflexivity.
-Qed.
-
-(* Generated language: *)
-
-Definition generates {Q E} (G:@DFA Q E) w : Prop :=
-  ~ extended_transition G (proper_state (initial_state G)) w = sink_state.
-
-Theorem prefix_closed: forall {Q E} (G:@DFA Q E) w w',
-    generates G (w ++ w') -> generates G w.
-Proof.
-  unfold generates, not.
-  intros Q E G w w' H0 H1.
-  rewrite dist_extended_transition in H0.
-  rewrite H1 in H0.
-  apply H0.
-  destruct w'; reflexivity.
-Qed.
-
+Definition transition (q:nat) (e:event) :=
+  match q, e with
+    0%nat, add => 5%nat |
+    0%nat, rem => 1%nat |
+    1%nat, add => 2%nat |
+    2%nat, rem => 3%nat |
+    3%nat, add => 4%nat |
+    4%nat, rem => 1%nat |
+    5%nat, add => 1%nat |
+      _  ,  _  => 10%nat
+  end.
+(* Axiom transition : nat->event->nat. *)
