QueueingSystems.v
@@ -1,359 +1,43 @@
-Require Import Coq.Lists.List.
-Import ListNotations.
-Set Implicit Arguments.
-Require Import DFA.
-
+Require Import Coq.Init.Nat Coq.Lists.List Omega Utils DFA.
+Import ListNotations Coq.Bool.Bool.
 Require BinIntDef.
-Require Import Omega.
 Local Open Scope Z_scope.
 
-Axiom E : Type.
-Inductive event := add | rem | other (e : E).
-Definition E' := event.
-Axiom Q : Type.
-Axiom G : @DFA Q E'.
-Definition q0 := initial_state G.
-Definition pq0 := proper_state q0.
-Definition transition := transition G.
-Definition is_proper_transition q e := exists q',
-  proper_state q' = transition q e.
-Definition xtransition := extended_transition G.
-Definition ixtransition := xtransition pq0.
-Definition generates w := ~ ixtransition w = sink_state.
+Fixpoint verify_upper_bound' (q:nat) (m:Z) (s:list Z) (n:nat) :=
+  match n with O => s | S n =>
 
-Lemma ixtransition_nil__pq0: ixtransition [] = pq0.
-Proof. auto. Qed.
+    if (states_num <=? q)%nat then
+        Return valid s
+    else if nth q s (-1) =? -1 then
+        let s' := change s q m in
+        Return max3_lists (verify_upper_bound' (transition q add) (m+1) s' n)
+                          (verify_upper_bound' (transition q rem) (m-1) s' n)
+                          (verify_upper_bound' (transition q oth)   m   s' n)
+    else if nth q s (-1) >=? m then
+        Return valid s
+    else
+        Return invalid s
 
-Lemma extended_transition__transition: forall q e,
-  xtransition (proper_state q) [e] = transition q e.
-Proof. apply DFA.extended_transition__transition. Qed.
-Lemma transition_sink_state: forall w,
-  xtransition sink_state w = sink_state.
-Proof. apply DFA.transition_sink_state. Qed.
-Lemma dist_xtransition: forall w w' q,
-  xtransition q (w ++ w') = xtransition (xtransition q w) w'.
-Proof. apply DFA.dist_extended_transition. Qed.
-Lemma dist_ixtransition: forall w w',
-  ixtransition (w ++ w') = xtransition (ixtransition w) w'.
-Proof. unfold ixtransition. intros w w'. apply dist_xtransition. Qed.
-Theorem prefix_closed: forall w w',
-  generates (w ++ w') -> generates w.
-Proof. apply DFA.prefix_closed. Qed.
-
-Definition count_event (e : E') :=
-  match e with
-    add => 1  |
-    rem => -1 |
-    other e' => 0
   end.
 
-Fixpoint count_buffer w :=
-  match w with
-    [] => 0 |
-    e::w' => count_event e + count_buffer w'
+Fixpoint verify_upper_bound'' (q:nat) (m:Z) (s:list Z) (n:nat) :=
+  match n with O => s | S n =>
+
+    if (states_num <=? q)%nat then
+        Return valid s
+    else if nth q s (-1) =? -1 then
+        let s'   := change s q m in
+        let s''  := verify_upper_bound'' (transition q add) (m+1) s'  n in
+        let s''' := verify_upper_bound'' (transition q oth)   m   s'' n in
+        Return max3_lists s'' s''' (verify_upper_bound'' (transition q rem) (m-1) s''' n)
+    else if nth q s (-1) >=? m then
+        Return valid s
+    else
+        Return invalid s
+
   end.
 
-Lemma dist_count_buffer: forall w1 w2,
-  count_buffer (w1 ++ w2) = count_buffer w1 + count_buffer w2.
-Proof.
-  intros w1 w2.
-  induction w1 as [|e w1 IHw1].
-  - auto.
-  - simpl. rewrite IHw1. omega.
-Qed.
+Definition verify_upper_bound :=
+  extract_invalid (verify_upper_bound'' 0 0 (initial_solution states_num) (states_num+2)) [].
 
-Lemma dist_count_buffer': forall w e,
-  count_buffer (w ++ [e]) = count_buffer w + count_event e.
-Proof.
-  intros w e.
-  induction w as [|e' w IH]; simpl; try (rewrite IH); omega.
-Qed.
-
-Axiom n0 : Z.
-Axiom n : Z.
-
-Definition is_upper_bounded := forall w, generates w -> n0 + count_buffer w <= n.
-
-Definition is_tangible q := exists w,
-  proper_state q = ixtransition w.
-
-Lemma buffer_count_leq_f: forall f,
-  ( f(pq0) = n0 /\ forall q, is_tangible q -> forall e,
-    is_proper_transition q e ->
-      f(transition q e) >= f(proper_state q) + count_event e ) ->
-  forall w, generates w -> n0 + count_buffer w <= f(ixtransition w).
-Proof.
-  intros f [H H0] w H1.
-  induction w as [|e w IHw] using @rev_ind.
-  - simpl.
-    rewrite ixtransition_nil__pq0.
-    omega.
-  - pose H1 as H2; apply prefix_closed in H2.
-    apply IHw in H2.
-    rewrite dist_ixtransition.
-    rewrite dist_count_buffer'.
-    remember (ixtransition w) as q eqn:eq_q.
-    destruct q.
-    {
-      apply prefix_closed in H1.
-      unfold generates in H1.
-      symmetry in eq_q.
-      contradiction.
-    }
-    remember (xtransition (proper_state q) [e]) as q' eqn:eq_q'; destruct q' as [|q'].
-    + unfold generates in H1; rewrite dist_ixtransition in H1.
-      symmetry in eq_q'.
-      rewrite eq_q in eq_q'.
-      contradiction.
-    + assert (H3: proper_state q' = transition q e).
-      { rewrite extended_transition__transition in eq_q'; auto. }
-      assert (f (proper_state q') >= f (proper_state q) + count_event e).
-      {
-        rewrite H3.
-        apply H0.
-        - exists w. auto.
-        - exists q'. auto.
-      }
-      omega.
-Qed.
-
-Theorem upper_bound1:
-  ( exists f, f(pq0) = n0 /\ forall q, is_tangible q ->
-    f(proper_state q) <= n /\ ( forall e, is_proper_transition q e ->
-      f(transition q e) >= f(proper_state q) + count_event e ) ) ->
-  is_upper_bounded.
-Proof.
-  unfold is_upper_bounded.
-  intros [f [H H0]] w H1.
-  assert (H2: n0 + count_buffer w <= f(ixtransition w)).
-  { apply buffer_count_leq_f; try split; try (apply H0); auto. }
-  assert (f (ixtransition w) <= n).
-  {
-    destruct (ixtransition w) as [|q] eqn:eq.
-    - contradiction.
-    - destruct H0 with (q:=q); try (exists w); auto.
-  }
-  omega.
-Qed.
-
-Notation " w ~> q " := (ixtransition w = q) (at level 60).
-
-Lemma g2__generates: forall w q,
-  w ~> (proper_state q) -> generates w.
-Proof.
-  unfold generates, not.
-  intros w q H H0.
-  rewrite H in H0.
-  discriminate.
-Qed.
-
-Lemma not_nil_if_count: forall w,
-  count_buffer w > 0 -> w <> [].
-Proof.
-  unfold not.
-  intros w H H0.
-  destruct w.
-  - inversion H.
-  - discriminate.
-Qed.
-
-Lemma cycle: forall q,
-  forall w, xtransition q w = q -> xtransition q (w++w) = q.
-Proof.
-  intros q w H.
-  rewrite dist_xtransition.
-  rewrite H.
-  auto.
-Qed.
-
-Fixpoint word_pow (w:list E') (n:nat) :=
-  match n with
-    O => [] |
-    S n => w ++ (word_pow w n)
-  end.
-
-Theorem count_word_pow: forall w n,
-  count_buffer (word_pow w n) = (Z.of_nat n) * (count_buffer w).
-Proof.
-  intros w n.
-  induction n as [|n IHn].
-  - auto.
-  - replace (word_pow w (S n)) with (w ++ word_pow w n).
-    rewrite dist_count_buffer.
-    rewrite IHn.
-    rewrite Nat2Z.inj_succ, <- Zmult_succ_l_reverse.
-    omega.
-    auto.
-Qed.
-
-Lemma q0_cycle: forall w n,
-  w ~> pq0 -> (word_pow w n) ~> pq0.
-Proof.
-  intros w n H.
-  induction n as [|n IHn].
-  - auto.
-  - simpl.
-    rewrite dist_ixtransition.
-    rewrite H.
-    auto.
-Qed.
-
-Lemma q0_cycle_count: forall w n,
-  (count_buffer w > 0 /\ w ~> pq0) ->
-  exists w', w' ~> pq0 /\ count_buffer w' > n.
-Proof.
-  intros w n [H H0].
-  destruct n eqn:eq_n.
-  - exists w. auto.
-  - exists (word_pow w ((Pos.to_nat p)+1)).
-    split.
-    + apply q0_cycle.
-      auto.
-    + rewrite count_word_pow.
-      assert (Z.pos p > 0). { apply Zgt_pos_0. }
-      assert (Z.pos p + 1 <= Z.of_nat (Pos.to_nat p + 1) * count_buffer w).
-      {
-        replace (Z.pos p + 1) with ((Z.pos p + 1)*1); try omega.
-        apply Zmult_le_compat; try omega.
-        rewrite Z.add_1_r. replace ((Pos.to_nat p + 1)%nat) with ((S (Pos.to_nat p))); try omega.
-        simpl.
-        rewrite Zpos_P_of_succ_nat.
-        rewrite positive_nat_Z.
-        simpl.
-        omega.
-      }
-      omega.
-  - exists w.
-    split.
-    + auto.
-    + rewrite <- eq_n.
-      assert (n < 0). { rewrite eq_n. apply Zlt_neg_0. }
-      omega.
-Qed.
-
-Lemma q0_cycle_no_upper_bound:
-  (exists w, w ~> pq0 /\ count_buffer w > 0) -> ~ is_upper_bounded.
-Proof.
-  unfold is_upper_bounded, not.
-  intros [w [H H0]] H1.
-  assert (H2: count_buffer w > 0 /\ w ~> pq0). auto.
-  apply q0_cycle_count with(n:=(n-n0)) in H2.
-  destruct H2 as [w' [H2 H3]].
-  apply g2__generates, H1 in H2.
-  omega.
-Qed.
-
-Definition state_upper_bound q m :=
-  forall w, w ~> q -> n0 + count_buffer w <= m.
-
-Definition min_state_upper_bound q m :=
-  state_upper_bound q m /\ ~ state_upper_bound q (m-1).
-
-Theorem q0_n0_bounded: is_upper_bounded -> min_state_upper_bound pq0 n0.
-Proof.
-  unfold min_state_upper_bound, state_upper_bound.
-  intro H.
-  split.
-  - intros w H0.
-    destruct (count_buffer w) eqn:eq_count.
-    + omega.
-    + assert (count_buffer w > 0). { rewrite eq_count. apply Zgt_pos_0. }
-      assert (exists w, w ~> pq0 /\ count_buffer w > 0). { exists w. auto. }
-      apply q0_cycle_no_upper_bound in H2.
-      contradiction.
-    + assert (Z.neg p < 0). { apply Zlt_neg_0. }
-      omega.
-  - unfold not. intro H0.
-    assert (H1: [] ~> pq0). { auto. }
-    apply H0 in H1.
-    simpl in H1.
-    omega.
-Qed.
-
-Lemma transition_upper_bound: forall q m1 m2 e,
-  is_tangible q -> min_state_upper_bound (proper_state q) m1 ->
-  min_state_upper_bound (transition q e) m1 -> m2 >= m1 + count_event e.
-Proof.
-Admitted.
-
-Axiom func_choice : forall A B (R : A -> B -> Prop),
-  (forall x, exists y, R x y) -> exists f, forall x, R x (f x).
-
-Definition f'_prop pq m := forall q,
-  pq = proper_state q -> is_tangible q -> state_upper_bound pq m.
-
-Lemma f'_def:
-  is_upper_bounded -> exists f, forall q, f'_prop q (f q).
-Proof.
-  intro H.
-  apply func_choice.
-  intro q.
-  exists n.
-  intros q' H0 H1 w H2.
-  rewrite H0 in H2.
-  apply g2__generates in H2.
-  unfold is_upper_bounded in H.
-  apply H in H2.
-  auto.
-Qed.
-
-Definition f_prop pq m := forall q,
-  pq = proper_state q -> is_tangible q -> min_state_upper_bound pq m.
-
-Lemma f'__f:
-  (exists f, forall q, f'_prop q (f q)) ->
-  exists f, forall q, f_prop q (f q).
-Proof.
-  intros [f H].
-  apply func_choice.
-  intro q.
-
-Lemma f_def:
-  is_upper_bounded -> exists f, forall q, f_prop q (f q).
-Proof.
-  intro H.
-  apply func_choice.
-  unfold f_prop.
-  intro q.
-Admitted.
-
-Lemma f_unicity: forall q m1 m2,
-  min_state_upper_bound q m1 -> min_state_upper_bound q m2 -> m1 = m2.
-Proof.
-Admitted.
-
-Theorem upper_bound2:
-  is_upper_bounded ->
-  ( exists f, f(pq0) = n0 /\ forall q, is_tangible q ->
-    f(proper_state q) <= n /\ ( forall e, is_proper_transition q e ->
-      f(transition q e) >= f(proper_state q) + count_event e ) ).
-Proof.
-  intro H.
-  pose H as H0; apply f_def in H0; destruct H0 as [f H0].
-  unfold f_prop in H0.
-  exists f.
-  split.
-  - destruct H0 with (q:=pq0) (q0:=q0); try (exists []); auto.
-    apply q0_n0_bounded in H.
-    apply f_unicity with (q:=pq0); unfold min_state_upper_bound; auto.
-  - intros q H1.
-    split.
-    + 
-Admitted.
-
-Theorem upper_bound:
-  ( exists f, f(pq0) = n0 /\ forall q, is_tangible q ->
-    f(proper_state q) <= n /\ ( forall e, is_proper_transition q e ->
-      f(transition q e) >= f(proper_state q) + count_event e ) ) <->
-  is_upper_bounded.
-Proof.
-  split. apply upper_bound1. apply upper_bound2.
-Qed.
-
-
-
-
-
-
-
-
+Compute verify_upper_bound.
