Utils.v
@@ -1,0 +1,53 @@
+Require Import Coq.Init.Nat Coq.Lists.List Omega.
+Import ListNotations Coq.Bool.Bool.
+Require BinIntDef.
+Local Open Scope Z_scope.
+
+Definition Return {A} a:A := a.
+
+Fixpoint change {A} (l:list A) (n:nat) (a:A) :=
+  match l, n with
+    x::l, S n => x::change l n a |
+    x::l,  O  => a::l            |
+     l  ,  _  => l
+  end.
+
+Fixpoint initial_solution' (n:nat) :=
+  match n with
+     O    => []                         |
+    S n   => initial_solution' n ++ [-1]
+  end.
+
+Definition initial_solution n := initial_solution' n ++ [1].
+
+Fixpoint valid (s:list Z) :=
+  match s with
+    x::[] => [0]        |
+    x::l  => x::valid l |
+    []    => []
+  end.
+
+Fixpoint invalid (s:list Z) :=
+  match s with
+    x::[] => [1]          |
+    x::l  => x::invalid l |
+    []    => []
+  end.
+
+Definition max3 (a b c:Z) :=
+  if (a >=? b) && (a >=? c) then a
+  else if (b >=? a) && (b >=? c) then b
+  else c.
+
+Fixpoint max3_lists (l1 l2 l3:list Z) :=
+  match l1, l2, l3 with
+    x1::l1, x2::l2, x3::l3 => max3 x1 x2 x3::max3_lists l1 l2 l3 |
+      _   ,   _   ,    _   => []
+  end.
+
+Fixpoint extract_invalid (l1 l2:list Z) :=
+  match l1 with
+    x::[] => if x =? 0 then (l2, true) else (l2, false) |
+    x::l1 => extract_invalid l1 (l2 ++ [x])             |
+      []  => (l2, false)
+  end.
